theories/modules/SModTr.v
@@ -137,7 +137,7 @@ Module SModTr. Section HOARE.
     interpV (handle img sp) it.
 
   Definition trans_body : (bool * sp_type * option fspec) → fbody → fbody :=
-    λ '(img, sp, fsp) bd, HoareFun fsp (trans img sp ∘ bd).
+    λ '(img, sp, fsp) bd, HoareFun fsp (trans (* img *) (is_some fsp) sp ∘ bd).
 
   Definition trans_ktree sp (sb : fnsem_type (option fspec * fbody)) : fnsem_type fbody :=
     map_snd (λ '(fsp, bd), trans_body (sb.1.1.1, if sb.1.1.1 then sp else sp_none, fsp) bd) sb.
